%Jennifer Pan, August 2011

\documentclass[10pt,letter]{article}
	% basic article document class
	% use percent signs to make comments to yourself -- they will not show up.

\usepackage{amsmath}
\usepackage{amssymb}
	% packages that allow mathematical formatting

\usepackage[final]{graphicx}
\usepackage{caption}
\usepackage{subcaption}
\usepackage{subcaption}
	% package that allows you to include graphics
\usepackage{tikz}
\usepackage{setspace}
	% package that allows you to change spacing

\onehalfspacing
	% text become 1.5 spaced

\usepackage{fullpage}
	% package that specifies normal margins

\renewcommand{\vector}[1]{\boldsymbol{#1}}
\newcommand{\problem}[1]{\section*{Problem #1}}
\newcommand{\problempart}[1]{\paragraph{#1}}

\begin{document}
	% line of code telling latex that your document is beginning


\title{ECON 511 Problem Set 9}

\author{Nicholas Wu}

\date{Spring 2021}
	% Note: when you omit this command, the current dateis automatically included

\maketitle
	% tells latex to follow your header (e.g., title, author) commands.
%\textbf{Note:} I use bold symbols to denote vectors and nonbolded symbols to denote scalars. I primarily use vector notation to shorthand some of the sums, since many of the sums are dot products.

\problem{1}

\problempart{1}
The firm problem is
\[ \max P(s^t)A_t(s^t)N_t(s^t) - W_t(s^t)N_t(s^t) \]
so the FOC is
\[ P(s^t)A_t(s^t) = W_t(s^t) \]
\problempart{2}
The consumer problem is
\[ \max \sum_{t=0}^{\infty} \beta^t \sum_{s^t}\pi(s^t)\left(\log C_t(s^t) + \log\left(\frac{M_t(s^t)}{P_t(s^t)} \right) - \frac{N_t(s^t)^{1+\varphi}}{1+\varphi} \right)\]
subject to
\[P_t(s^t) C_t(s^t) + M_t(s^t)+ Q_t(s^t)B_t(s^t) \le M_{t-1}(s^{t-1}) + B_{t-1}(s^{t-1}) + W_t(s^t)N_t(s^t) - T_t(s^t) \]
so the Lagrangian is
\[\sum_{t=0}^{\infty} \beta^t \sum_{s^t}\pi(s^t)\left(\log C_t(s^t) + \log\left(\frac{M_t(s^t)}{P_t(s^t)} \right) - \frac{N_t(s^t)^{1+\varphi}}{1+\varphi} \right)\]\[- \lambda_t(s^t)(P_t(s^t) C_t(s^t) + M_t(s^t)+ Q_t(s^t)B_t(s^t) - M_{t-1}(s^{t-1}) - B_{t-1}(s^{t-1}) - W_t(s^t)N_t(s^t) + T_t(s^t))  \]
The FOCs are then
\[ \beta^t\frac{\pi(s^t)}{C_t(s^t)} = \lambda_t(s^t)P_t(s^t) \]
\[ \beta^t\pi(s^t) N_t(s^t)^\varphi = \lambda_t(s^t)W_t(s^t) \]
\[ \lambda_t(s^t) Q_t(s^t) = \sum_{s^{t+1}} \lambda_{t+1}(s^{t+1}) \]
\[ \beta^t\frac{\pi(s^t)}{M_t(s^t)} = \lambda_t(s^t) - \sum_{s^{t+1}}\lambda_{t+1}(s^{t+1}) \]
\problempart{3}
Eliminating $\lambda_t(s^t)$, we get
\[ \beta^t\pi(s^t) N_t(s^t)^\varphi = \beta^t\frac{\pi(s^t)}{C_t(s^t)P_t(s^t)}W_t(s^t) \]
\[  N_t(s^t)^\varphi = \frac{W_t(s^t)}{C_t(s^t)P_t(s^t)} \]
For $Q$, we get
\[ \beta^t\frac{\pi(s^t)}{C_t(s^t)P_t(s^t)} Q_t(s^t) = \sum_{s^{t+1}} \beta^{t+1}\frac{\pi(s^{t+1})}{C_{t+1}(s^{t+1})P_{t+1}(s^{t+1})} \]
\[ \frac{\pi(s^t)Q_t(s^t)}{C_t(s^t)P_t(s^t)}  = \sum_{s^{t+1}} \frac{\beta\pi(s^{t+1})}{C_{t+1}(s^{t+1})P_{t+1}(s^{t+1})} \]
\[ Q_t(s^t)  = \sum_{s^{t+1}} \frac{\beta\pi(s^{t+1}|s_t)C_t(s^t)P_t(s^t)}{C_{t+1}(s^{t+1})P_{t+1}(s^{t+1})} \]
\[ Q_t(s^t)  = E_{t} \frac{\beta C_t(s^t)P_t(s^t)}{C_{t+1}(s^{t+1})P_{t+1}(s^{t+1})} \]
and for $M$, we have
\[ \beta^t\frac{\pi(s^t)}{M_t(s^t)} = \beta^t\frac{\pi(s^t)}{C_t(s^t)P_t(s^t)} - \sum_{s^{t+1}} \frac{\beta^{t+1}\pi(s^{t+1})}{C_{t+1}(s^{t+1})P_{t+1}(s^{t+1})}  \]
\[ \frac{1}{M_t(s^t)} = \frac{1}{C_t(s^t)P_t(s^t)} - \sum_{s^{t+1}} \frac{\beta\pi(s^{t+1}|s^t)}{C_{t+1}(s^{t+1})P_{t+1}(s^{t+1})}  \]
\[ \frac{1}{M_t(s^t)} = \frac{1}{C_t(s^t)P_t(s^t)} - E_t \frac{\beta}{C_{t+1}(s^{t+1})P_{t+1}(s^{t+1})}  \]
\[ \frac{1}{M_t(s^t)} = \frac{1- Q_t(s^t)}{C_t(s^t)P_t(s^t)}   \]
\problempart{4}
From market clearing, we have
\[ A_t(s^t)N_t(s^t) = C_t(s^t) \]
From the firm FOC
\[ P(s^t)A_t(s^t) = W_t(s^t) \]
From the previous part
\[  N_t(s^t)^\varphi = \frac{W_t(s^t)}{C_t(s^t)P_t(s^t)} \]
so
\[  N_t(s^t)^\varphi = \frac{P(s^t)A_t(s^t)}{C_t(s^t)P_t(s^t)} = \frac{A_t(s^t)}{C_t(s^t)} = \frac{1}{N_t(s^t)} \]
\[ N_t(s^t)^{\varphi+1} = 1 \]
\[ (1 + \varphi)\log N_t = 0 \]
\[ n_t = 0 \]
Since
\[ A_t(s^t)N_t(s^t) = C_t(s^t) \]
\[ \log A_t(s^t) + \log N_t(s^t) = \log C_t(s^t) \]
\[ a_t + n_t = c_t \]
\[ a_t = c_t \]
And since $Y_t = C_t$, by market clearing, $y_t = c_t = a_t$.
\problempart{5}
Log linearizing, we get
\[ \varphi n_t = w_t - c_t - p_t  \]
\[ Q_t(s^t)  = E_{t} \frac{\beta C_t(s^t)P_t(s^t)}{C_{t+1}(s^{t+1})P_{t+1}(s^{t+1})} \]
\[ -i_t = -\rho -  E_t(p_{t+1} - p_t) - E_t(c_{t+1} - c_t)  \]
\[ c_t = \rho - i_t + E_t\pi_{t+1} + E_t c_{t+1} \]
\[ m_t = c_t + p_t - \log(1-Q_t)\]

\problempart{6}
From a constant velocity of money, we get
\[ p_t + c_t - m_t = p_{t-1} + c_{t-1} - m_{t-1} \]
\[ \pi_t + c_t - c_{t-1} + m_{t-1} - m_t = 0 \]
\[ \pi_t + a_t - a_{t-1} + m_{t-1} - m_t = 0 \]
\[ \pi_t + \ln(1 + \gamma_a) - \ln(1 + \gamma_m) + \epsilon_a^t - \epsilon_m^t \]
\[ \pi_t = \ln(1 + \gamma_m) - \ln(1 + \gamma_a) + \epsilon_m^t - \epsilon_a^t \]
Plugging into Euler eq
\[ c_t = \rho + i_t - E_t\pi_{t+1} - E_t c_{t+1} \]
\[ = \rho - i_t + E_t\left(\ln(1 + \gamma_m) - \ln(1 + \gamma_a) + \epsilon_m^t - \epsilon_a^t \right) + E_t c_{t+1} \]
\[ = \rho - i_t + \ln(1 + \gamma_m) - \ln(1 + \gamma_a) + E_t c_{t+1} \]
\[ = \rho - i_t + \ln(1 + \gamma_m) - \ln(1 + \gamma_a) + E_t a_{t+1} \]
\[ = \rho - i_t + \ln(1 + \gamma_m) - \ln(1 + \gamma_a) + a_t + \ln(1 + \gamma_a) \]
\[ = \rho - i_t + \ln(1 + \gamma_m) + a_t  \]
Since $c_t = a_t$,
\[ \rho - i_t + \ln(1 + \gamma_m)  = 0 \]
\[ i_t = \rho + \ln(1 + \gamma_m) \]
Now, since
\[ \frac{1}{M_t(s^t)} = \frac{1- Q_t(s^t)}{C_t(s^t)P_t(s^t)}   \]
\[ V  = \frac{PY}{M} = \frac{PC}{M} = 1 - Q \approx i_t = \rho + \ln(1+ \gamma_m) \]
as desired.
\problempart{7}
By constant velocity of money,
\[ p_t + c_t - m_t = \log V \approx \log (\rho + \ln(1+ \gamma_m)) \]
Since money only factors into the utility via $m_t - p_t = \log (M_t/P_t)$ we have that
\[  m_t - p_t = a_t - \log V \approx \log (\rho + \ln(1+ \gamma_m)) \]
So only $\gamma_m$ affects the utility.

\problempart{8}
The social planner problem is
\[ \max \ln C_t + \ln \frac{M_t}{P_t} - \frac{N_t^{1+\varphi}}{1+ \varphi} \]
subject to $C_t = A_tN_t$. The FOC in $M$ gives
\[ \frac{1}{M} = 0 \]
From before we hhave
\[ 0 = \frac{1}{M} = \frac{1-Q}{PC} \]
\[ 0 = \frac{PC}{M} = 1-Q = i \]
Hence $i_t = 0$.


\problem{2}

\problempart{1}
Plugging into the EE:
\[ \hat{Y}_t = E_t \hat{Y}_{t+1} - \sigma(\hat{i}_t - E_t \hat{\pi}_{t+1} - \hat{r}_t^n) \]
\[ \hat{Y}_t = E_t \hat{Y}_{t+1} - \sigma(\phi_y \hat{Y}_t + \phi_r \hat{r}^n_t - E_t \hat{\pi}_{t+1} - \hat{r}_t^n) \]
\[ \hat{Y}_t = E_t \hat{Y}_{t+1} - \sigma \phi_y \hat{Y}_t - \sigma  \phi_r \hat{r}^n_t + \sigma  E_t \hat{\pi}_{t+1} + \sigma  \hat{r}_t^n \]
\[ (1 + \sigma\phi_y)\hat{Y}_t = E_t \hat{Y}_{t+1} + \sigma  E_t \hat{\pi}_{t+1} + \sigma (1 - \phi_r)  \hat{r}_t^n \]
\[ (1 + \sigma\phi_y)\hat{Y}_t - E_t \hat{Y}_{t+1} - \sigma (1 - \phi_r)  \hat{r}_t^n =  \sigma  E_t \hat{\pi}_{t+1}  \]
\[  E_t \hat{\pi}_{t+1}= \frac{1 + \sigma\phi_y}{\sigma}\hat{Y}_t - \frac{1}{\sigma}E_t \hat{Y}_{t+1} -  (1 - \phi_r)  \hat{r}_t^n     \]
Then we can take any arbitrary random $\delta_{t}$ such that $E_t \delta_{t+1} = 0$, and if
\[ \hat{\pi}_{t+1}= \frac{1 + \sigma\phi_y}{\sigma}\hat{Y}_t - \frac{1}{\sigma}E_t \hat{Y}_{t+1} -  (1 - \phi_r)  \hat{r}_t^n + \delta_{t+1} \]
So there cannot be a unique solution.
\problempart{2}
From the hint, we take
\[ \hat{i}_t = r_t + E_t \hat{\pi}_{t+1} \]
\[ \hat{i}_{t+1} = \phi_i \hat{i}_t + \phi_\pi \hat{\pi}_{t+1} \]
\[ E_t \hat{i}_{t+1} = \phi_i \hat{i}_t + \phi_\pi E_t \hat{\pi}_{t+1} \]
\[  E_t \hat{i}_{t+1} - \phi_i \hat{i}_t = \phi_\pi E_t \hat{\pi}_{t+1} \]
\[ \hat{i}_t = r_t + \frac{1}{\phi_\pi}E_t \hat{i}_{t+1} - \frac{\phi_i}{\phi_\pi} \hat{i}_t \]
\[  \frac{\phi_\pi + \phi_i}{\phi_\pi} \hat{i}_t = r_t + \frac{1}{\phi_\pi}E_t \hat{i}_{t+1} \]
\[   \hat{i}_t = \frac{\phi_\pi}{\phi_\pi + \phi_i}r_t + \frac{1}{\phi_\pi + \phi_i}E_t \hat{i}_{t+1} \]
\[   \hat{i}_t = \left(\frac{1}{\phi_\pi + \phi_i}\right)^T E_t \hat{i}_{t+T}+ \sum_{\tau = t}^{T} \frac{\phi_\pi}{(\phi_\pi + \phi_i)^{\tau - t+1}}r_{\tau} \]
For a unique solution, we need $|\phi_\pi + \phi_i| > 1$.
\problempart{3}
From the EE, we have
\[ \hat{i}_t = r_t + E_t \hat{\pi}_{t+1} \]
\[ \phi_\pi E_t \hat{\pi}_{t+1}  = r_t + E_t \hat{\pi}_{t+1} \]
\[ (\phi_\pi-1) E_t \hat{\pi}_{t+1}  = r_t  \]
\[ E_t \hat{\pi}_{t+1}  = \frac{1}{\phi_\pi - 1}r_t  \]
Then as part 1, we can take some $\delta_t$ such that $E_t\delta_{t+1} = 0$,
\[ \hat{\pi}_{t+1} = \frac{1}{\phi_\pi - 1}r_t + \delta_{t+1} \]
If $\phi_\pi = 1$, then $r = 0$, which is not possible. Hence all allowable values of $\phi_\pi$, there is no unique bounded solution.
\end{document}
	% line of code telling latex that your document is ending. If you leave this out, you'll get an error
